src/mqtt-packet-parser/src/ffi.c
@@ -1,0 +1,15 @@
+#include <stdio.h>
+#include <stdint.h>
+#include "kremlib.h"
+
+void print_hex(uint8_t i) {
+  printf("%02x", i);
+}
+
+C_String_t topic_name_uint8_to_c_string(uint8_t *u8_buffer) {
+  return (char *)u8_buffer;
+}
+
+C_String_t payload_uint8_to_c_string(uint8_t *u8_buffer, uint32_t min_packet_size, uint32_t max_packet_size, uint32_t n) {
+  return (char *)u8_buffer;
+}
