src/mqtt-packet-parser/src/ffi.fst
@@ -1,16 +1,11 @@
-module Utils
+module FFI
 
-open FStar.HyperStack.ST
 module U8 = FStar.UInt8
 module U32 = FStar.UInt32
 module B = LowStar.Buffer
-module HS = FStar.HyperStack
 
-let zero_terminated_buffer_u8 (h: HS.mem) (b: B.buffer U8.t) =
-  let s = B.as_seq h b in
-  B.length b > 0 /\
-  B.length b <= FStar.UInt.max_int 32 /\
-  U8.v (Seq.index s (B.length b - 1)) = 0
+open FStar.HyperStack.ST
+open Common
 
 assume val print_hex (i:U8.t): Stack unit
   (requires (fun h -> true))
