src/mqtt-packet-parser/src/common.fst
@@ -1,0 +1,475 @@
+module Common
+
+module U8 = FStar.UInt8
+module U32 = FStar.UInt32
+module B = LowStar.Buffer
+module HS = FStar.HyperStack
+
+open FStar.HyperStack.ST
+open LowStar.BufferOps
+open FStar.Int.Cast
+open C.String
+
+
+open Const
+
+val is_valid_decoding_packet_check: ptr_for_decoding_packets: B.buffer U8.t
+  -> bytes_length: (v:U8.t{U8.v v >= 1 && U8.v v <= 4})
+  -> Stack (v:U8.t{U8.v v <= 3})
+    (requires fun h0 -> B.live h0 ptr_for_decoding_packets /\ B.length ptr_for_decoding_packets = 4)
+    (ensures fun h0 r h1 -> true)
+let is_valid_decoding_packet_check ptr_for_decoding_packets bytes_length =
+  push_frame ();
+  let ptr_status: B.buffer (status:U8.t{U8.v status <= 3}) = B.alloca 0uy 1ul in
+  let inv h (i: nat) =
+    B.live h ptr_status /\
+    B.live h ptr_for_decoding_packets
+     in
+  let body (i: U32.t{ 0 <= U32.v i && U32.v i < 4 }): Stack unit
+    (requires (fun h -> inv h (U32.v i)))
+    (ensures (fun _ _ _ -> true))
+  =
+    let ptr_status_v: (status:U8.t{U8.v status <= 3}) = ptr_status.(0ul) in
+    let bytes_length_u32: U32.t = uint8_to_uint32(bytes_length) in
+      if (U8.eq ptr_status_v 0uy) then
+        (
+          if (U32.lt i bytes_length_u32) then
+            (
+              let decoding_packet: U8.t = ptr_for_decoding_packets.(i) in
+                if (U8.eq bytes_length 1uy) then
+                  (
+                    if (U8.lt decoding_packet 0uy || U8.gt decoding_packet 127uy) then
+                      (
+                        ptr_status.(0ul) <- 1uy
+                      )
+                  )
+                else
+                  (
+                    let data_length_minus_one: U32.t = uint8_to_uint32 (U8.sub bytes_length 1uy) in
+                    if (U32.eq i data_length_minus_one) then
+                      (
+                        if (U8.lt decoding_packet 1uy || U8.gt decoding_packet 127uy) then
+                          (
+                            ptr_status.(0ul) <- 2uy
+                          )
+                      ) else
+                        (
+                          if (U8.lt decoding_packet 128uy || U8.gt decoding_packet max_u8) then
+                            (
+                              ptr_status.(0ul) <- 3uy
+                            )
+                        )
+                  )
+            )
+        )
+  in
+  C.Loops.for 0ul 4ul inv body;
+  let r: (status:U8.t{U8.v status <= 3}) = ptr_status.(0ul) in
+  pop_frame ();
+  r
+
+val most_significant_four_bit_to_zero: i:U8.t -> y:U8.t{U8.v y >= 0 && U8.v y <= 127}
+let most_significant_four_bit_to_zero i =
+    if (U8.(i >=^ 128uy)) then
+      U8.(i -^ 128uy)
+    else
+      i
+
+val except_most_significant_four_bit_to_zero: i:U8.t -> y:U8.t{U8.v y = 0 || U8.v y = 128}
+let except_most_significant_four_bit_to_zero i =
+    if (U8.(i <=^ 127uy)) then
+      0uy
+    else
+      128uy
+
+val decodeing_variable_bytes: ptr_for_decoding_packets: B.buffer U8.t
+  -> bytes_length:U8.t{U8.v bytes_length >= 1 && U8.v bytes_length <= 4}
+  -> Stack (remaining_length:type_remaining_length)
+    (requires fun h0 -> B.live h0 ptr_for_decoding_packets  /\ B.length ptr_for_decoding_packets = 4)
+    (ensures fun h0 r h1 -> true)
+let decodeing_variable_bytes ptr_for_decoding_packets bytes_length =
+  push_frame ();
+  let ptr_for_decoding_packet: B.buffer U8.t = B.alloca 0uy 1ul in
+  let ptr_for_remaining_length: B.buffer type_remaining_length = B.alloca 0ul 1ul in
+  let ptr_status: B.buffer (status:U8.t{U8.v status <= 1}) = B.alloca 1uy 1ul in
+  let ptr_temp1 : B.buffer (temp: U32.t{U32.v temp <= 127}) = B.alloca 0ul 1ul in
+  let ptr_temp2 : B.buffer (temp: U32.t{U32.v temp <= 16383}) = B.alloca 0ul 1ul in
+  let ptr_temp3 : B.buffer (temp: U32.t{U32.v temp <= 2097151}) = B.alloca 0ul 1ul in
+  let ptr_temp4 : B.buffer type_remaining_length = B.alloca 0ul 1ul in
+  let inv h (i: nat) = B.live h ptr_for_decoding_packets /\
+    B.live h ptr_for_decoding_packet /\
+    B.live h ptr_for_remaining_length /\
+    B.live h ptr_status /\
+    B.live h ptr_temp1 /\
+    B.live h ptr_temp2 /\
+    B.live h ptr_temp3 /\
+    B.live h ptr_temp4
+     in
+  let is_valid_decoding_packet: (v:U8.t{U8.v v <= 3}) = is_valid_decoding_packet_check ptr_for_decoding_packets bytes_length in
+  if (is_valid_decoding_packet <> 0uy) then
+    (
+      pop_frame ();
+      max_u32
+    )
+  else
+    (
+      let body (i: U32.t{ 0 <= U32.v i && U32.v i <= 3 }): Stack unit
+        (requires (fun h -> inv h (U32.v i)))
+        (ensures (fun _ _ _ -> true))
+      =
+        let ptr_status_v: (status:U8.t{U8.v status <= 1}) = ptr_status.(0ul) in
+          if (ptr_status_v = 1uy) then
+            (
+              let decoding_packet: U8.t = ptr_for_decoding_packets.(i) in
+
+              let b_u8: (x:U8.t{U8.v x >= 0 && U8.v x <= 127}) =
+                most_significant_four_bit_to_zero decoding_packet in
+
+              let b_u32: (x:U32.t{U32.v x >= 0 && U32.v x <= 127}) = uint8_to_uint32 b_u8 in
+              let b2_u8: (x:U8.t{U8.v x = 0 || U8.v x = 128}) =
+                except_most_significant_four_bit_to_zero decoding_packet in
+
+              if (i = 0ul) then
+                (
+                  ptr_temp1.(0ul) <- U32.(b_u32 *^ 1ul);
+                  ptr_for_remaining_length.(0ul) <- ptr_temp1.(0ul)
+                )
+              else if (i = 1ul) then
+                (
+                    ptr_temp2.(0ul) <- U32.(ptr_temp1.(0ul) +^ b_u32 *^ 128ul);
+                    ptr_for_remaining_length.(0ul) <- ptr_temp2.(0ul)
+                )
+              else if (i = 2ul) then
+                (
+                    ptr_temp3.(0ul) <- U32.(ptr_temp2.(0ul) +^ (b_u32 *^ 128ul *^ 128ul));
+                    ptr_for_remaining_length.(0ul) <- ptr_temp3.(0ul)
+                )
+              else
+                (
+                    ptr_temp4.(0ul) <- U32.(ptr_temp3.(0ul) +^ (b_u32 *^ 128ul *^ 128ul *^ 128ul));
+                    ptr_for_remaining_length.(0ul) <- ptr_temp4.(0ul)
+                );
+
+              if (b2_u8 = 0uy) then
+                ptr_status.(0ul) <- 0uy
+            )
+      in
+      C.Loops.for 0ul 4ul inv body;
+      let remaining_length: type_remaining_length =
+        ptr_for_remaining_length.(0ul) in
+      pop_frame ();
+      remaining_length
+  )
+
+val get_remaining_length: bytes_length:U8.t{U8.v bytes_length >= 1 && U8.v bytes_length <= 4} -> ptr_for_decoding_packets: B.buffer U8.t -> packet_size: type_packet_size
+  -> Stack (remaining_length:type_remaining_length)
+  (requires fun h0 -> B.live h0 ptr_for_decoding_packets /\ B.length ptr_for_decoding_packets = 4)
+  (ensures fun _ _ _ -> true)
+let get_remaining_length bytes_length ptr_for_decoding_packets packet_size =
+  let fixed_value: U32.t = U32.(packet_size -^ 1ul) in
+  let bytes_length_u32: U32.t = uint8_to_uint32(bytes_length) in
+  let r: type_remaining_length =
+    let untrust_r: type_remaining_length =
+      decodeing_variable_bytes ptr_for_decoding_packets bytes_length in
+    (
+      if (untrust_r <> max_u32) then
+        (
+          if (U32.(bytes_length_u32 +^ untrust_r) = fixed_value) then
+            untrust_r
+          else
+            max_u32
+        )
+      else
+        max_u32
+    ) in r
+
+val get_message_type: message_type_bits: U8.t -> type_mqtt_control_packets_restrict
+let get_message_type message_type_bits =
+  if (U8.lt message_type_bits 1uy || U8.gt message_type_bits 15uy) then
+    max_u8
+  else
+    message_type_bits
+
+val is_valid_flag: s:struct_fixed_header_constant -> flag: type_flag_restrict -> bool
+let is_valid_flag s flag = U8.eq s.flags_constant.flag flag
+
+val get_struct_fixed_header_constant_except_publish :
+  (message_type: type_mqtt_control_packets_restrict)
+  -> struct_fixed_header_constant
+let get_struct_fixed_header_constant_except_publish message_type =
+  if (U8.eq message_type define_mqtt_control_packet_CONNECT) then
+    {
+      message_type_constant = define_mqtt_control_packet_CONNECT;
+      message_name_constant = define_mqtt_control_packet_CONNECT_label;
+      flags_constant = {
+        flag = define_flag_CONNECT;
+        dup_flag = max_u8;
+        qos_flag = max_u8;
+        retain_flag = max_u8;
+      };
+    }
+  else if (U8.eq message_type define_mqtt_control_packet_CONNACK) then
+      {
+        message_type_constant = define_mqtt_control_packet_CONNACK;
+        message_name_constant = define_mqtt_control_packet_CONNACK_label;
+        flags_constant = {
+          flag = define_flag_CONNACK;
+          dup_flag = max_u8;
+          qos_flag = max_u8;
+          retain_flag = max_u8;
+        };
+      }
+  else if (U8.eq message_type define_mqtt_control_packet_PUBACK) then
+    {
+      message_type_constant = define_mqtt_control_packet_PUBACK;
+      message_name_constant = define_mqtt_control_packet_PUBACK_label;
+      flags_constant = {
+        flag = define_flag_PUBACK;
+        dup_flag = max_u8;
+        qos_flag = max_u8;
+        retain_flag = max_u8;
+      };
+    }
+  else if (U8.eq message_type define_mqtt_control_packet_PUBREC) then
+    {
+      message_type_constant = define_mqtt_control_packet_PUBREC;
+      message_name_constant = define_mqtt_control_packet_PUBREC_label;
+      flags_constant = {
+        flag = define_flag_PUBREC;
+        dup_flag = max_u8;
+        qos_flag = max_u8;
+        retain_flag = max_u8;
+      };
+    }
+  else if (U8.eq message_type define_mqtt_control_packet_PUBREL) then
+    {
+      message_type_constant = define_mqtt_control_packet_PUBREL;
+      message_name_constant = define_mqtt_control_packet_PUBREL_label;
+      flags_constant = {
+        flag = define_flag_PUBREL;
+        dup_flag = max_u8;
+        qos_flag = max_u8;
+        retain_flag = max_u8;
+      };
+    }
+  else if (U8.eq message_type define_mqtt_control_packet_PUBCOMP) then
+    {
+      message_type_constant = define_mqtt_control_packet_PUBCOMP;
+      message_name_constant = define_mqtt_control_packet_PUBCOMP_label;
+      flags_constant = {
+        flag = define_flag_PUBCOMP;
+        dup_flag = max_u8;
+        qos_flag = max_u8;
+        retain_flag = max_u8;
+      };
+    }
+  else if (U8.eq message_type define_mqtt_control_packet_SUBSCRIBE) then
+    {
+      message_type_constant = define_mqtt_control_packet_SUBSCRIBE;
+      message_name_constant = define_mqtt_control_packet_SUBSCRIBE_label;
+      flags_constant = {
+        flag = define_flag_SUBSCRIBE;
+        dup_flag = max_u8;
+        qos_flag = max_u8;
+        retain_flag = max_u8;
+      };
+    }
+  else if (U8.eq message_type define_mqtt_control_packet_SUBACK) then
+    {
+      message_type_constant = define_mqtt_control_packet_SUBACK;
+      message_name_constant = define_mqtt_control_packet_SUBACK_label;
+      flags_constant = {
+        flag = define_flag_SUBACK;
+        dup_flag = max_u8;
+        qos_flag = max_u8;
+        retain_flag = max_u8;
+      };
+    }
+  else if (U8.eq message_type define_mqtt_control_packet_UNSUBSCRIBE) then
+    {
+      message_type_constant = define_mqtt_control_packet_UNSUBSCRIBE;
+      message_name_constant = define_mqtt_control_packet_UNSUBSCRIBE_label;
+      flags_constant = {
+        flag = define_flag_UNSUBSCRIBE;
+        dup_flag = max_u8;
+        qos_flag = max_u8;
+        retain_flag = max_u8;
+      };
+    }
+  else if (U8.eq message_type define_mqtt_control_packet_UNSUBACK) then
+    {
+      message_type_constant = define_mqtt_control_packet_UNSUBACK;
+      message_name_constant = define_mqtt_control_packet_UNSUBACK_label;
+      flags_constant = {
+        flag = define_flag_UNSUBACK;
+        dup_flag = max_u8;
+        qos_flag = max_u8;
+        retain_flag = max_u8;
+      };
+    }
+  else if (U8.eq message_type define_mqtt_control_packet_PINGREQ) then
+    {
+      message_type_constant = define_mqtt_control_packet_PINGREQ;
+      message_name_constant = define_mqtt_control_packet_PINGREQ_label;
+      flags_constant = {
+        flag = define_flag_PINGREQ;
+        dup_flag = max_u8;
+        qos_flag = max_u8;
+        retain_flag = max_u8;
+      };
+    }
+  else if (U8.eq message_type define_mqtt_control_packet_PINGRESP) then
+    {
+      message_type_constant = define_mqtt_control_packet_PINGRESP;
+      message_name_constant = define_mqtt_control_packet_PINGRESP_label;
+      flags_constant = {
+        flag = define_flag_PINGRESP;
+        dup_flag = max_u8;
+        qos_flag = max_u8;
+        retain_flag = max_u8;
+      };
+    }
+  else if (U8.eq message_type define_mqtt_control_packet_DISCONNECT) then
+    {
+      message_type_constant = define_mqtt_control_packet_DISCONNECT;
+      message_name_constant = define_mqtt_control_packet_DISCONNECT_label;
+      flags_constant = {
+        flag = define_flag_DISCONNECT;
+        dup_flag = max_u8;
+        qos_flag = max_u8;
+        retain_flag = max_u8;
+      };
+    }
+  else
+    {
+      message_type_constant = define_mqtt_control_packet_AUTH;
+      message_name_constant = define_mqtt_control_packet_AUTH_label;
+      flags_constant = {
+        flag = define_flag_AUTH;
+        dup_flag = max_u8;
+        qos_flag = max_u8;
+        retain_flag = max_u8;
+      };
+    }
+
+val error_struct_fixed_header:
+  (error_struct: struct_error_struct)
+  -> struct_fixed_header
+let error_struct_fixed_header error_struct = {
+    message_type = max_u8;
+    message_name = !$"";
+    flags = {
+      flag = max_u8;
+      dup_flag = max_u8;
+      qos_flag = max_u8;
+      retain_flag = max_u8;
+    };
+    remaining_length = max_u32;
+    connect = {
+      protocol_name = !$"";
+      protocol_version = max_u8;
+      flags = {
+        connect_flag = max_u8;
+        user_name = max_u8;
+        password = max_u8;
+        will_retain = max_u8;
+        will_qos = max_u8;
+        will_flag = max_u8;
+        clean_start = max_u8;
+      };
+      keep_alive = max_u32;
+      connect_topic_length = max_u32;
+      connect_property = {
+        connect_property_id = max_u8;
+        connect_property_name = !$"";
+      }
+    };
+    publish = {
+      topic_length = max_u32;
+      topic_name = !$"";
+      property_length = max_u32;
+      payload = !$"";
+    };
+    disconnect = {
+      disconnect_reason_code = max_u8;
+      disconnect_reason_code_name = !$"";
+    };
+    error = error_struct;
+  }
+
+let zero_terminated_buffer_u8 (h: HS.mem) (b: B.buffer U8.t) =
+  let s = B.as_seq h b in
+  B.length b > 0 /\
+  B.length b <= FStar.UInt.max_int 32 /\
+  U8.v (Seq.index s (B.length b - 1)) = 0
+
+val slice_byte:
+  byte:U8.t
+  -> a:U8.t{U8.v a <= 7}
+  -> b:U8.t {U8.v b <= 8 && U8.v a < U8.v b} -> U8.t
+let slice_byte byte a b =
+  let for_mask_temp1: U8.t =
+    (
+      if (U32.eq 0ul (uint8_to_uint32 a)) then
+        0b11111111uy
+      else if (U32.eq 1ul (uint8_to_uint32 a)) then
+        0b01111111uy
+      else if (U32.eq 2ul (uint8_to_uint32 a)) then
+        0b00111111uy
+      else if (U32.eq 3ul (uint8_to_uint32 a)) then
+        0b00011111uy
+      else if (U32.eq 4ul (uint8_to_uint32 a)) then
+        0b00001111uy
+      else if (U32.eq 5ul (uint8_to_uint32 a)) then
+        0b00000111uy
+      else if (U32.eq 6ul (uint8_to_uint32 a)) then
+        0b00000011uy
+      else
+        0b00000001uy
+    ) in
+  let for_mask_temp2: U8.t =
+    (
+      if (U32.eq 1ul (uint8_to_uint32 b)) then
+        0b10000000uy
+      else if (U32.eq 2ul (uint8_to_uint32 b)) then
+        0b11000000uy
+      else if (U32.eq 3ul (uint8_to_uint32 b)) then
+        0b11100000uy
+      else if (U32.eq 4ul (uint8_to_uint32 b)) then
+        0b11110000uy
+      else if (U32.eq 5ul (uint8_to_uint32 b)) then
+        0b11111000uy
+      else if (U32.eq 6ul (uint8_to_uint32 b)) then
+        0b11111100uy
+      else if (U32.eq 7ul (uint8_to_uint32 b)) then
+        0b11111110uy
+      else
+        0b11111111uy
+    ) in
+    let mask: U8.t = U8.logand for_mask_temp1 for_mask_temp2 in
+    let r: U8.t = U8.shift_right (U8.logand byte mask) (U32.sub 8ul (uint8_to_uint32 b)) in
+  r
+
+
+val get_flag: (message_type: type_mqtt_control_packets_restrict)
+  -> (fixed_header_first_one_byte: U8.t)
+  -> type_flag_restrict
+let get_flag message_type fixed_header_first_one_byte =
+  let v: U8.t = slice_byte fixed_header_first_one_byte 4uy 8uy in
+      if (U8.eq message_type define_mqtt_control_packet_PUBREL ||
+        U8.eq message_type define_mqtt_control_packet_SUBSCRIBE ||
+        U8.eq message_type define_mqtt_control_packet_UNSUBSCRIBE) then
+        (
+          if (v <> 0b0010uy) then
+            max_u8
+          else
+            v
+        )
+      else
+        (
+          if (v <> 0b0000uy) then
+            max_u8
+          else
+            v
+        )
+
