src/mqtt-packet-parser/src/connect.fst
@@ -1,0 +1,81 @@
+module Connect
+
+open Const
+open Common
+
+open C.String
+
+module U8 = FStar.UInt8
+
+val assemble_connect_struct: s: struct_connect_parts
+  -> Pure struct_fixed_header
+    (requires true)
+    (ensures (fun r -> true))
+let assemble_connect_struct s =
+  let connect_constant: struct_fixed_header_constant = s.connect_connect_constant in
+  let connect_flag: U8.t = s.connect_connect_flag in
+  let user_name_flag: U8.t = slice_byte connect_flag 0uy 1uy in
+  let password_flag: U8.t = slice_byte connect_flag 1uy 2uy in
+  let will_retain_flag: U8.t = slice_byte connect_flag 2uy 3uy in
+  let will_qos_flag: U8.t = slice_byte connect_flag 3uy 5uy in
+  let will_flag: U8.t = slice_byte connect_flag 5uy 6uy in
+  let clean_start_flag: U8.t = slice_byte connect_flag 6uy 7uy in
+  let resreved_flag: U8.t = slice_byte connect_flag 7uy 8uy in
+  let connect_property_id: U8.t = s.connect_connect_property_id in
+  {
+    message_type = connect_constant.message_type_constant;
+    message_name = connect_constant.message_name_constant;
+    flags = {
+      flag = connect_constant.flags_constant.flag;
+      dup_flag = connect_constant.flags_constant.dup_flag;
+      qos_flag = connect_constant.flags_constant.qos_flag;
+      retain_flag = connect_constant.flags_constant.retain_flag;
+    };
+    remaining_length = s.connect_remaining_length;
+    connect = 
+        {
+          protocol_name = !$"MQTT";
+          protocol_version = 5uy;
+          flags = {
+            connect_flag = connect_flag;
+            user_name = user_name_flag;
+            password = password_flag;
+            will_retain = will_retain_flag;
+            will_qos = will_qos_flag;
+            will_flag = will_flag;
+            clean_start = clean_start_flag;
+          };
+          keep_alive = s.connect_keep_alive;
+          connect_topic_length = s.connect_connect_topic_length;
+          connect_property =
+          if (U8.eq connect_property_id define_connect_property_session_expiry_interval_id) then 
+            define_struct_connect_property_session_expiry_interval
+          else if (U8.eq connect_property_id define_connect_property_receive_maximum_id) then 
+            define_struct_connect_property_receive_maximum
+          else if (U8.eq connect_property_id define_connect_property_maximum_packet_size_id) then 
+            define_struct_connect_property_maximum_packet_size
+          else if (U8.eq connect_property_id define_connect_property_topic_alias_maximum_id) then 
+            define_struct_connect_property_topic_alias_maximum
+          else if (U8.eq connect_property_id define_connect_property_request_response_information_id) then 
+            define_struct_connect_property_request_response_information
+          else if (U8.eq connect_property_id define_connect_property_request_problem_information_id) then 
+            define_struct_connect_property_request_problem_information    
+          else if (U8.eq connect_property_id define_connect_property_user_property_id) then 
+            define_struct_connect_property_user_property
+          else if (U8.eq connect_property_id define_connect_property_authentication_method_id) then 
+            define_struct_connect_property_authentication_method
+          else
+            define_struct_connect_property_authentication_data
+        };
+    publish = {
+      topic_length = max_u32;
+      topic_name = !$"";
+      property_length = max_u32;
+      payload = !$"";
+    };
+    disconnect = define_struct_disconnect_error;
+    error = {
+      code = define_no_error_code;
+      message = define_no_error;
+    };
+  }
