src/mqtt-packet-parser/src/const.fst
@@ -1,0 +1,627 @@
+module Const
+
+module U8 = FStar.UInt8
+module U32 = FStar.UInt32
+
+open C.String
+
+val max_u8: U8.t
+let max_u8 = 255uy
+
+val max_u32: U32.t
+let max_u32 = 4294967295ul
+
+val min_packet_size: U32.t
+let min_packet_size = 2ul
+
+val max_packet_size: U32.t
+let max_packet_size = 268435460ul
+
+val max_request_size: U32.t
+let max_request_size = 268435461ul
+
+val min_request_size: U32.t
+let min_request_size = 0ul
+
+val max_payload_size: U32.t
+let max_payload_size = 268435455ul
+
+type type_packet_size =
+  packet_size:
+    U32.t{U32.v packet_size >= U32.v min_packet_size && U32.v packet_size <= U32.v max_packet_size}
+
+type type_mqtt_control_packets = U8.t
+let define_mqtt_control_packet_CONNECT : type_mqtt_control_packets = 1uy
+let define_mqtt_control_packet_CONNACK : type_mqtt_control_packets = 2uy
+let define_mqtt_control_packet_PUBLISH : type_mqtt_control_packets = 3uy
+let define_mqtt_control_packet_PUBACK : type_mqtt_control_packets = 4uy
+let define_mqtt_control_packet_PUBREC : type_mqtt_control_packets = 5uy
+let define_mqtt_control_packet_PUBREL : type_mqtt_control_packets = 6uy
+let define_mqtt_control_packet_PUBCOMP : type_mqtt_control_packets = 7uy
+let define_mqtt_control_packet_SUBSCRIBE : type_mqtt_control_packets = 8uy
+let define_mqtt_control_packet_SUBACK : type_mqtt_control_packets = 9uy
+let define_mqtt_control_packet_UNSUBSCRIBE : type_mqtt_control_packets = 10uy
+let define_mqtt_control_packet_UNSUBACK : type_mqtt_control_packets = 11uy
+let define_mqtt_control_packet_PINGREQ : type_mqtt_control_packets = 12uy
+let define_mqtt_control_packet_PINGRESP : type_mqtt_control_packets = 13uy
+let define_mqtt_control_packet_DISCONNECT : type_mqtt_control_packets = 14uy
+let define_mqtt_control_packet_AUTH : type_mqtt_control_packets = 15uy
+
+type type_mqtt_control_packet_label = C.String.t
+let define_mqtt_control_packet_CONNECT_label : type_mqtt_control_packet_label = !$"CONNECT"
+let define_mqtt_control_packet_CONNACK_label : type_mqtt_control_packet_label = !$"CONNACK"
+let define_mqtt_control_packet_PUBLISH_label : type_mqtt_control_packet_label = !$"PUBLISH"
+let define_mqtt_control_packet_PUBACK_label : type_mqtt_control_packet_label = !$"PUBACK"
+let define_mqtt_control_packet_PUBREC_label : type_mqtt_control_packet_label = !$"PUBREC"
+let define_mqtt_control_packet_PUBREL_label : type_mqtt_control_packet_label = !$"PUBREL"
+let define_mqtt_control_packet_PUBCOMP_label : type_mqtt_control_packet_label = !$"PUBCOMP"
+let define_mqtt_control_packet_SUBSCRIBE_label : type_mqtt_control_packet_label = !$"SUBSCRIBE"
+let define_mqtt_control_packet_SUBACK_label : type_mqtt_control_packet_label = !$"SUBACK"
+let define_mqtt_control_packet_UNSUBSCRIBE_label : type_mqtt_control_packet_label = !$"UNSUBSCRIBE"
+let define_mqtt_control_packet_UNSUBACK_label : type_mqtt_control_packet_label = !$"UNSUBACK"
+let define_mqtt_control_packet_PINGREQ_label : type_mqtt_control_packet_label = !$"PINGREQ"
+let define_mqtt_control_packet_PINGRESP_label : type_mqtt_control_packet_label = !$"PINGRESP"
+let define_mqtt_control_packet_DISCONNECT_label : type_mqtt_control_packet_label = !$"DISCONNECT"
+let define_mqtt_control_packet_AUTH_label : type_mqtt_control_packet_label = !$"AUTH"
+type type_message_name_restrict =
+  v:type_mqtt_control_packet_label{
+    v = define_mqtt_control_packet_CONNECT_label ||
+    v = define_mqtt_control_packet_CONNACK_label ||
+    v = define_mqtt_control_packet_PUBLISH_label ||
+    v = define_mqtt_control_packet_PUBACK_label ||
+    v = define_mqtt_control_packet_PUBREC_label ||
+    v = define_mqtt_control_packet_PUBREL_label ||
+    v = define_mqtt_control_packet_PUBCOMP_label ||
+    v = define_mqtt_control_packet_SUBSCRIBE_label ||
+    v = define_mqtt_control_packet_SUBACK_label ||
+    v = define_mqtt_control_packet_UNSUBSCRIBE_label ||
+    v = define_mqtt_control_packet_UNSUBACK_label ||
+    v = define_mqtt_control_packet_PINGREQ_label ||
+    v = define_mqtt_control_packet_PINGRESP_label ||
+    v = define_mqtt_control_packet_DISCONNECT_label ||
+    v = define_mqtt_control_packet_AUTH_label ||
+    v = !$""
+  }
+
+
+type type_mqtt_control_packets_restrict =
+  v:type_mqtt_control_packets{U8.v v >= 1 && U8.v v <= 15 || U8.eq v max_u8}
+
+type type_remaining_length =
+  (remaining_length: U32.t{U32.v remaining_length <= U32.v (U32.sub max_packet_size 5ul) || U32.eq remaining_length max_u32})
+
+type type_flag_restrict =
+  flag: U8.t{
+    U8.eq flag 0b0000uy ||
+    U8.eq flag 0b0010uy ||
+    U8.eq flag max_u8
+}
+
+type type_dup_flags = U8.t
+let define_dup_flag_first_delivery : type_dup_flags = 0uy
+let define_dup_flag_re_delivery : type_dup_flags = 1uy
+
+type type_qos_flags = U8.t
+let define_qos_flag_at_most_once_delivery : type_qos_flags = 0b00uy
+let define_qos_flag_at_least_once_delivery : type_qos_flags = 0b01uy
+let define_qos_flag_exactly_once_delivery : type_qos_flags = 0b10uy
+
+type type_retain_flags = U8.t
+let define_retain_flag_must_not_store_application_message : type_retain_flags = 0uy
+let define_retain_flag_must_store_application_message : type_retain_flags = 1uy
+
+type type_dup_flags_restrict =
+  dup_flag: type_dup_flags{U8.v dup_flag <= 1 || U8.eq dup_flag max_u8}
+
+type type_qos_flags_restrict =
+  qos_flag: type_qos_flags{U8.v qos_flag <= 2 || U8.eq qos_flag max_u8}
+
+type type_retain_flags_restrict =
+  retain_flag: type_retain_flags{U8.v retain_flag <= 1 || U8.eq retain_flag max_u8}
+
+type type_flags = U8.t
+
+let define_flag_CONNECT : type_flags = 0b0000uy
+let define_flag_CONNACK : type_flags = 0b0000uy
+
+let define_flag_PUBACK : type_flags = 0b0000uy
+let define_flag_PUBREC : type_flags = 0b0000uy
+let define_flag_PUBREL : type_flags = 0b0010uy
+let define_flag_PUBCOMP : type_flags = 0b0000uy
+let define_flag_SUBSCRIBE : type_flags = 0b0010uy
+let define_flag_SUBACK : type_flags = 0b0000uy
+let define_flag_UNSUBSCRIBE : type_flags = 0b0010uy
+let define_flag_UNSUBACK : type_flags = 0b0000uy
+let define_flag_PINGREQ : type_flags = 0b0000uy
+let define_flag_PINGRESP : type_flags = 0b0000uy
+let define_flag_DISCONNECT : type_flags = 0b0000uy
+let define_flag_AUTH : type_flags = 0b0000uy
+
+type struct_flags = {
+  flag: type_flag_restrict;
+  dup_flag: type_dup_flags_restrict;
+  qos_flag: type_qos_flags_restrict;
+  retain_flag: type_retain_flags_restrict;
+}
+
+type struct_fixed_header_constant = {
+  message_type_constant: type_mqtt_control_packets_restrict;
+  message_name_constant: type_message_name_restrict;
+  flags_constant: struct_flags;
+}
+
+type struct_connect_flags = {
+      connect_flag: U8.t;
+      user_name: U8.t;
+      password: U8.t;
+      will_retain: U8.t;
+      will_qos: U8.t;
+      will_flag: U8.t;
+      clean_start: U8.t;
+  }
+
+type struct_connect_property = {
+    connect_property_id: U8.t;
+    connect_property_name: C.String.t;
+}
+
+let define_connect_property_session_expiry_interval_id: U8.t = 0x11uy
+let define_connect_property_receive_maximum_id: U8.t = 0x21uy
+let define_connect_property_maximum_packet_size_id: U8.t = 0x27uy
+let define_connect_property_topic_alias_maximum_id: U8.t = 0x22uy
+let define_connect_property_request_response_information_id: U8.t = 0x19uy
+let define_connect_property_request_problem_information_id: U8.t = 0x17uy
+let define_connect_property_user_property_id: U8.t = 0x26uy
+let define_connect_property_authentication_method_id: U8.t = 0x15uy
+let define_connect_property_authentication_data_id: U8.t = 0x16uy
+
+let define_struct_connect_property_session_expiry_interval: struct_connect_property =
+  {
+    connect_property_id = define_connect_property_session_expiry_interval_id;
+    connect_property_name = !$"Session Expiry Interval";
+  }
+
+let define_struct_connect_property_receive_maximum: struct_connect_property =
+  {
+    connect_property_id = define_connect_property_receive_maximum_id;
+    connect_property_name = !$"Receive Maximum";
+  }
+
+let define_struct_connect_property_maximum_packet_size: struct_connect_property =
+  {
+    connect_property_id = define_connect_property_maximum_packet_size_id;
+    connect_property_name = !$"Maximum Packet Size";
+  }
+
+let define_struct_connect_property_topic_alias_maximum: struct_connect_property =
+  {
+    connect_property_id = define_connect_property_topic_alias_maximum_id;
+    connect_property_name = !$"Topic Alias Maximum";
+  }
+
+let define_struct_connect_property_request_response_information: struct_connect_property =
+  {
+    connect_property_id = define_connect_property_request_response_information_id;
+    connect_property_name = !$"Request Response Information";
+  }
+
+let define_struct_connect_property_request_problem_information: struct_connect_property =
+  {
+    connect_property_id = define_connect_property_request_problem_information_id;
+    connect_property_name = !$"Request Problem Information";
+  }
+
+let define_struct_connect_property_user_property: struct_connect_property =
+  {
+    connect_property_id = define_connect_property_user_property_id;
+    connect_property_name = !$"User Property";
+  }
+
+let define_struct_connect_property_authentication_method: struct_connect_property =
+  {
+    connect_property_id = define_connect_property_authentication_method_id;
+    connect_property_name = !$"Authentication Method";
+  }
+
+let define_struct_connect_property_authentication_data: struct_connect_property =
+  {
+    connect_property_id = define_connect_property_authentication_data_id;
+    connect_property_name = !$"Authentication Data";
+  }
+
+// 3.1.2.3 Connect Flags
+type struct_connect = {
+  protocol_name: C.String.t;
+  protocol_version: U8.t;
+  flags: struct_connect_flags;
+  keep_alive: U32.t;
+  connect_topic_length: U32.t;
+  connect_property: struct_connect_property;
+}  
+
+type type_topic_name_restrict =
+  (
+    topic_name: C.String.t{U32.v (strlen topic_name) <= 65535}
+  )
+
+type type_topic_length_restrict =
+  (topic_length_restrict: U32.t{U32.v topic_length_restrict <= 65535 || U32.eq topic_length_restrict max_u32})
+
+type type_property_length = type_remaining_length
+
+type type_payload_restrict =
+  (
+    payload: C.String.t{U32.v (strlen payload) <= U32.v max_packet_size}
+  )
+
+type type_payload_offset = payload_offset: U32.t{U32.v payload_offset < U32.v max_packet_size}
+
+type struct_variable_header_publish = {
+  topic_length: type_topic_length_restrict;
+  topic_name: type_topic_name_restrict;
+  property_length: type_property_length;
+  payload: type_payload_restrict;
+}
+
+type type_disconnect_reason_code = U8.t
+let define_disconnect_reason_code_normal_disconnection: type_disconnect_reason_code = 0uy
+let define_disconnect_reason_code_disconnect_with_will_message: type_disconnect_reason_code = 4uy
+let define_disconnect_reason_code_unspecified_error: type_disconnect_reason_code = 128uy
+let define_disconnect_reason_code_malformed_packet: type_disconnect_reason_code = 129uy
+let define_disconnect_reason_code_protocol_error: type_disconnect_reason_code = 130uy
+let define_disconnect_reason_code_implementation_specific_error: type_disconnect_reason_code = 131uy
+let define_disconnect_reason_code_not_authorized: type_disconnect_reason_code = 135uy
+let define_disconnect_reason_code_server_busy: type_disconnect_reason_code = 137uy
+let define_disconnect_reason_code_server_shutting_down: type_disconnect_reason_code = 139uy
+let define_disconnect_reason_code_keep_alive_timeout: type_disconnect_reason_code = 141uy
+let define_disconnect_reason_code_session_taken_over: type_disconnect_reason_code = 142uy
+let define_disconnect_reason_code_topic_filter_invalid: type_disconnect_reason_code = 143uy
+let define_disconnect_reason_code_topic_name_invalid: type_disconnect_reason_code = 144uy
+let define_disconnect_reason_receive_maximum_exceeded: type_disconnect_reason_code = 147uy
+let define_disconnect_reason_topic_alias_invalid: type_disconnect_reason_code = 148uy
+let define_disconnect_reason_packet_too_large: type_disconnect_reason_code = 149uy
+let define_disconnect_reason_message_rate_too_high: type_disconnect_reason_code = 150uy
+let define_disconnect_reason_quota_exceeded: type_disconnect_reason_code = 151uy
+let define_disconnect_reason_administrative_action: type_disconnect_reason_code = 152uy
+let define_disconnect_reason_payload_format_invalid: type_disconnect_reason_code = 153uy
+let define_disconnect_reason_retain_not_supported: type_disconnect_reason_code = 154uy
+let define_disconnect_reason_qos_not_supported: type_disconnect_reason_code = 155uy
+let define_disconnect_reason_use_another_server: type_disconnect_reason_code = 156uy
+let define_disconnect_reason_server_moved: type_disconnect_reason_code = 157uy
+let define_disconnect_reason_shared_subscriptions_not_supported: type_disconnect_reason_code = 158uy
+let define_disconnect_reason_connection_rate_exceeded: type_disconnect_reason_code = 159uy
+let define_disconnect_reason_maximum_connect_time: type_disconnect_reason_code = 160uy
+let define_disconnect_reason_subscription_identifiers_not_supported: type_disconnect_reason_code = 161uy
+let define_disconnect_reason_wildcard_subscriptions_not_supported: type_disconnect_reason_code = 162uy
+
+type type_disconnect_reason_code_name = C.String.t
+let define_disconnect_reason_code_normal_disconnection_name: type_disconnect_reason_code_name = !$"Normal disconnection" 
+let define_disconnect_reason_code_disconnect_with_will_message_name: type_disconnect_reason_code_name = !$"Disconnect with Will Message"
+let define_disconnect_reason_code_unspecified_error_name: type_disconnect_reason_code_name = !$"Unspecified error"
+let define_disconnect_reason_code_malformed_packet_name: type_disconnect_reason_code_name = !$"Malformed Packet"
+let define_disconnect_reason_code_protocol_error_name: type_disconnect_reason_code_name = !$"Protocol Error"
+let define_disconnect_reason_code_implementation_specific_error_name: type_disconnect_reason_code_name = !$"Implementation specific error"
+let define_disconnect_reason_code_not_authorized_name: type_disconnect_reason_code_name = !$"Not authorized"
+let define_disconnect_reason_code_server_busy_name: type_disconnect_reason_code_name = !$"Server busy"
+let define_disconnect_reason_code_server_shutting_down_name: type_disconnect_reason_code_name = !$"Server shutting down"
+let define_disconnect_reason_code_keep_alive_timeout_name: type_disconnect_reason_code_name = !$"Keep Alive timeout"
+let define_disconnect_reason_code_session_taken_over_name: type_disconnect_reason_code_name = !$"Session taken over"
+let define_disconnect_reason_code_topic_filter_invalid_name: type_disconnect_reason_code_name = !$"Topic Filter invalid"
+let define_disconnect_reason_code_topic_name_invalid_name: type_disconnect_reason_code_name = !$"Topic Name invalid"
+let define_disconnect_reason_receive_maximum_exceeded_name: type_disconnect_reason_code_name = !$"Receive Maximum exceeded"
+let define_disconnect_reason_topic_alias_invalid_name: type_disconnect_reason_code_name = !$"Topic Alias invalid"
+let define_disconnect_reason_packet_too_large_name: type_disconnect_reason_code_name = !$"Packet too large"
+let define_disconnect_reason_message_rate_too_high_name: type_disconnect_reason_code_name = !$"Message rate too high"
+let define_disconnect_reason_quota_exceeded_name: type_disconnect_reason_code_name = !$"Quota exceeded"
+let define_disconnect_reason_administrative_action_name: type_disconnect_reason_code_name = !$"Administrative action"
+let define_disconnect_reason_payload_format_invalid_name: type_disconnect_reason_code_name = !$"Payload format invalid"
+let define_disconnect_reason_retain_not_supported_name: type_disconnect_reason_code_name = !$"Retain not supported"
+let define_disconnect_reason_qos_not_supported_name: type_disconnect_reason_code_name = !$"QoS not supported"
+let define_disconnect_reason_use_another_server_name: type_disconnect_reason_code_name = !$"Use another server"
+let define_disconnect_reason_server_moved_name: type_disconnect_reason_code_name = !$"Server moved"
+let define_disconnect_reason_shared_subscriptions_not_supported_name: type_disconnect_reason_code_name = !$"Shared Subscriptions not supported"
+let define_disconnect_reason_connection_rate_exceeded_name: type_disconnect_reason_code_name = !$"Connection rate exceeded"
+let define_disconnect_reason_maximum_connect_time_name: type_disconnect_reason_code_name = !$"Maximum connect time"
+let define_disconnect_reason_subscription_identifiers_not_supported_name: type_disconnect_reason_code_name = !$"Subscription Identifiers not supported"
+let define_disconnect_reason_wildcard_subscriptions_not_supported_name: type_disconnect_reason_code_name = !$"Wildcard Subscriptions not supported"
+
+type struct_disconnect_reason = {
+  disconnect_reason_code: type_disconnect_reason_code;
+  disconnect_reason_code_name: type_disconnect_reason_code_name;
+}
+
+let define_struct_disconnect_normal_disconnection: struct_disconnect_reason =
+  {
+    disconnect_reason_code = define_disconnect_reason_code_normal_disconnection;
+    disconnect_reason_code_name = define_disconnect_reason_code_normal_disconnection_name;
+  }
+
+let define_struct_disconnect_disconnect_with_will_message: struct_disconnect_reason =
+  {
+    disconnect_reason_code = define_disconnect_reason_code_disconnect_with_will_message;
+    disconnect_reason_code_name = define_disconnect_reason_code_disconnect_with_will_message_name;
+  }
+
+let define_struct_disconnect_unspecified_error: struct_disconnect_reason =
+  {
+    disconnect_reason_code = define_disconnect_reason_code_unspecified_error;
+    disconnect_reason_code_name = define_disconnect_reason_code_unspecified_error_name;
+  }
+
+let define_struct_disconnect_malformed_packet: struct_disconnect_reason =
+  {
+    disconnect_reason_code = define_disconnect_reason_code_malformed_packet;
+    disconnect_reason_code_name = define_disconnect_reason_code_malformed_packet_name;
+  }
+
+let define_struct_disconnect_protocol_error: struct_disconnect_reason =
+  {
+    disconnect_reason_code = define_disconnect_reason_code_protocol_error;
+    disconnect_reason_code_name = define_disconnect_reason_code_protocol_error_name;
+  }
+
+let define_struct_disconnect_implementation_specific_error: struct_disconnect_reason =
+  {
+    disconnect_reason_code = define_disconnect_reason_code_implementation_specific_error;
+    disconnect_reason_code_name = define_disconnect_reason_code_implementation_specific_error_name;
+  }
+
+let define_struct_disconnect_not_authorized: struct_disconnect_reason =
+  {
+    disconnect_reason_code = define_disconnect_reason_code_not_authorized;
+    disconnect_reason_code_name = define_disconnect_reason_code_not_authorized_name;
+  }
+
+let define_struct_disconnect_server_busy: struct_disconnect_reason =
+  {
+    disconnect_reason_code = define_disconnect_reason_code_server_busy;
+    disconnect_reason_code_name = define_disconnect_reason_code_server_busy_name;
+  }
+
+let define_struct_disconnect_server_shutting_down: struct_disconnect_reason =
+  {
+    disconnect_reason_code = define_disconnect_reason_code_server_shutting_down;
+    disconnect_reason_code_name = define_disconnect_reason_code_server_shutting_down_name;
+  }
+
+let define_struct_disconnect_keep_alive_timeout: struct_disconnect_reason =
+  {
+    disconnect_reason_code = define_disconnect_reason_code_keep_alive_timeout;
+    disconnect_reason_code_name = define_disconnect_reason_code_keep_alive_timeout_name;
+  }  
+
+let define_struct_disconnect_session_taken_over: struct_disconnect_reason =
+  {
+    disconnect_reason_code = define_disconnect_reason_code_session_taken_over;
+    disconnect_reason_code_name = define_disconnect_reason_code_session_taken_over_name;
+  } 
+
+let define_struct_disconnect_topic_filter_invalid: struct_disconnect_reason =
+  {
+    disconnect_reason_code = define_disconnect_reason_code_topic_filter_invalid;
+    disconnect_reason_code_name = define_disconnect_reason_code_topic_filter_invalid_name;
+  } 
+
+let define_struct_disconnect_topic_name_invalid: struct_disconnect_reason =
+  {
+    disconnect_reason_code = define_disconnect_reason_code_topic_name_invalid;
+    disconnect_reason_code_name = define_disconnect_reason_code_topic_name_invalid_name;
+  } 
+
+let define_struct_disconnect_receive_maximum_exceeded: struct_disconnect_reason =
+  {
+    disconnect_reason_code = define_disconnect_reason_receive_maximum_exceeded;
+    disconnect_reason_code_name = define_disconnect_reason_receive_maximum_exceeded_name;
+  } 
+
+let define_struct_disconnect_topic_alias_invalid: struct_disconnect_reason =
+  {
+    disconnect_reason_code = define_disconnect_reason_topic_alias_invalid;
+    disconnect_reason_code_name = define_disconnect_reason_topic_alias_invalid_name;
+  } 
+
+let define_struct_disconnect_packet_too_large: struct_disconnect_reason =
+  {
+    disconnect_reason_code = define_disconnect_reason_packet_too_large;
+    disconnect_reason_code_name = define_disconnect_reason_packet_too_large_name;
+  }   
+
+let define_struct_disconnect_message_rate_too_high: struct_disconnect_reason =
+  {
+    disconnect_reason_code = define_disconnect_reason_message_rate_too_high;
+    disconnect_reason_code_name = define_disconnect_reason_message_rate_too_high_name;
+  }   
+
+let define_struct_disconnect_quota_exceeded: struct_disconnect_reason =
+  {
+    disconnect_reason_code = define_disconnect_reason_quota_exceeded;
+    disconnect_reason_code_name = define_disconnect_reason_quota_exceeded_name;
+  }   
+
+let define_struct_disconnect_administrative_action: struct_disconnect_reason =
+  {
+    disconnect_reason_code = define_disconnect_reason_administrative_action;
+    disconnect_reason_code_name = define_disconnect_reason_administrative_action_name;
+  }   
+
+let define_struct_disconnect_payload_format_invalid: struct_disconnect_reason =
+  {
+    disconnect_reason_code = define_disconnect_reason_payload_format_invalid;
+    disconnect_reason_code_name = define_disconnect_reason_payload_format_invalid_name;
+  }   
+
+let define_struct_disconnect_retain_not_supported: struct_disconnect_reason =
+  {
+    disconnect_reason_code = define_disconnect_reason_retain_not_supported;
+    disconnect_reason_code_name = define_disconnect_reason_retain_not_supported_name;
+  }   
+
+let define_struct_disconnect_qos_not_supported: struct_disconnect_reason =
+  {
+    disconnect_reason_code = define_disconnect_reason_qos_not_supported;
+    disconnect_reason_code_name = define_disconnect_reason_qos_not_supported_name;
+  }   
+
+let define_struct_disconnect_use_another_server: struct_disconnect_reason =
+  {
+    disconnect_reason_code = define_disconnect_reason_use_another_server;
+    disconnect_reason_code_name = define_disconnect_reason_use_another_server_name;
+  }   
+
+let define_struct_disconnect_server_moved: struct_disconnect_reason =
+  {
+    disconnect_reason_code = define_disconnect_reason_server_moved;
+    disconnect_reason_code_name = define_disconnect_reason_server_moved_name;
+  }   
+
+let define_struct_disconnect_shared_subscriptions_not_supported: struct_disconnect_reason =
+  {
+    disconnect_reason_code = define_disconnect_reason_shared_subscriptions_not_supported;
+    disconnect_reason_code_name = define_disconnect_reason_shared_subscriptions_not_supported_name;
+  }   
+
+let define_struct_disconnect_connection_rate_exceeded: struct_disconnect_reason =
+  {
+    disconnect_reason_code = define_disconnect_reason_connection_rate_exceeded;
+    disconnect_reason_code_name = define_disconnect_reason_connection_rate_exceeded_name;
+  } 
+
+let define_struct_disconnect_maximum_connect_time: struct_disconnect_reason =
+  {
+    disconnect_reason_code = define_disconnect_reason_maximum_connect_time;
+    disconnect_reason_code_name = define_disconnect_reason_maximum_connect_time_name;
+  } 
+
+let define_struct_disconnect_subscription_identifiers_not_supported: struct_disconnect_reason =
+  {
+    disconnect_reason_code = define_disconnect_reason_subscription_identifiers_not_supported;
+    disconnect_reason_code_name = define_disconnect_reason_subscription_identifiers_not_supported_name;
+  } 
+
+let define_struct_disconnect_wildcard_subscriptions_not_supported: struct_disconnect_reason =
+  {
+    disconnect_reason_code = define_disconnect_reason_wildcard_subscriptions_not_supported;
+    disconnect_reason_code_name = define_disconnect_reason_wildcard_subscriptions_not_supported_name;
+  } 
+
+let define_struct_disconnect_error: struct_disconnect_reason =
+  {
+    disconnect_reason_code = max_u8;
+    disconnect_reason_code_name = !$"";
+  }
+
+
+type type_error_code = U8.t
+let define_no_error_code: type_error_code = 0uy
+let define_error_remaining_length_invalid_code: type_error_code = 1uy
+let define_error_message_type_invalid_code: type_error_code = 2uy
+let define_error_flag_invalid_code: type_error_code = 3uy
+let define_error_dup_flag_invalid_code: type_error_code = 4uy
+let define_error_qos_flag_invalid_code: type_error_code = 5uy
+let define_error_retain_flag_invalid_code: type_error_code = 6uy
+let define_error_topic_length_invalid_code: type_error_code = 7uy
+let define_error_topic_name_dont_zero_terminated_code: type_error_code = 8uy
+let define_error_property_length_invalid_code: type_error_code = 9uy
+let define_error_payload_invalid_code: type_error_code = 10uy
+let define_error_topic_name_have_inavlid_character_code: type_error_code = 11uy
+let define_error_protocol_name_invalid_code: type_error_code = 12uy
+let define_error_protocol_version_invalid_code: type_error_code = 13uy
+let define_error_connect_flag_invalid_code: type_error_code = 14uy
+
+type type_error_code_restrict =
+  (v:
+    type_error_code{
+      v = define_no_error_code ||
+      v = define_error_remaining_length_invalid_code ||
+      v = define_error_message_type_invalid_code ||
+      v = define_error_flag_invalid_code ||
+      v = define_error_dup_flag_invalid_code ||
+      v = define_error_qos_flag_invalid_code ||
+      v = define_error_retain_flag_invalid_code ||
+      v = define_error_topic_length_invalid_code ||
+      v = define_error_topic_name_dont_zero_terminated_code ||
+      v = define_error_topic_name_have_inavlid_character_code ||
+      v = define_error_property_length_invalid_code ||
+      v = define_error_payload_invalid_code ||
+      v = define_error_protocol_name_invalid_code ||
+      v = define_error_protocol_version_invalid_code ||
+      v = define_error_connect_flag_invalid_code
+    }
+  )
+
+type type_error_message = C.String.t
+let define_error_remaining_length_invalid: type_error_message = !$"remaining_length is invalid."
+let define_error_message_type_invalid: type_error_message = !$"message_type is invalid."
+let define_error_flag_invalid: type_error_message = !$"flag is invalid."
+let define_error_dup_flag_invalid: type_error_message = !$"dup_flag is invalid."
+let define_error_qos_flag_invalid: type_error_message = !$"qos_flag is invalid."
+let define_error_retain_flag_invalid: type_error_message = !$"retain_flag is invalid."
+let define_error_topic_length_invalid: type_error_message = !$"topic_length is invalid."
+let define_error_topic_name_dont_zero_terminated: type_error_message = !$"topic_name is not zero-terminated."
+let define_error_topic_name_have_inavlid_character: type_error_message = !$"topic_name have invalid character."
+let define_error_property_length_invalid: type_error_message = !$"property_length is invalid."
+let define_error_payload_invalid: type_error_message = !$"payload is invalid."
+let define_error_protocol_name_invalid: type_error_message = !$"protocol name is invalid."
+let define_error_protocol_version_invalid: type_error_message = !$"protocol version is invalid."
+let define_error_connect_flag_invalid: type_error_message = !$"connect flag is invalid."
+let define_no_error: type_error_message = !$""
+
+type type_error_message_restrict =
+  (v:
+    type_error_message{
+      v = define_no_error ||
+      v = define_error_remaining_length_invalid ||
+      v = define_error_message_type_invalid ||
+      v = define_error_flag_invalid ||
+      v = define_error_dup_flag_invalid ||
+      v = define_error_qos_flag_invalid ||
+      v = define_error_retain_flag_invalid ||
+      v = define_error_topic_length_invalid ||
+      v = define_error_topic_name_dont_zero_terminated ||
+      v = define_error_topic_name_have_inavlid_character ||
+      v = define_error_property_length_invalid ||
+      v = define_error_payload_invalid ||
+      v = define_error_protocol_name_invalid ||
+      v = define_error_protocol_version_invalid ||
+      v = define_error_connect_flag_invalid
+    }
+  )
+
+type struct_error_struct = {
+  code: type_error_code_restrict;
+  message: type_error_message_restrict;
+}
+
+type struct_fixed_header = {
+  message_type: type_mqtt_control_packets_restrict;
+  message_name: type_message_name_restrict;
+  flags: struct_flags;
+  remaining_length: type_remaining_length;
+  connect: struct_connect;
+  publish: struct_variable_header_publish;
+  disconnect: struct_disconnect_reason;
+  error: struct_error_struct;
+}
+
+type struct_publish_parts = {
+  publish_remaining_length: type_remaining_length;
+  publish_fixed_header_first_one_byte: U8.t;
+  publish_topic_name: type_topic_name_restrict;
+  publish_topic_length: type_topic_length_restrict;
+  publish_property_length: type_property_length;
+  publish_payload: type_payload_restrict;
+}
+
+type struct_connect_parts = {
+  connect_remaining_length: type_remaining_length;
+  connect_connect_constant: struct_fixed_header_constant;
+  connect_connect_flag: U8.t;
+  connect_keep_alive: U32.t;
+  connect_connect_topic_length: U32.t;
+  connect_connect_property_id: U8.t;
+}
+
+type struct_disconnect_parts = {
+  disconnect_remaining_length: type_remaining_length;
+  disconnect_disconnect_constant: struct_fixed_header_constant;
+}
