src/mqtt-packet-parser/src/disconnect.fst
@@ -1,0 +1,141 @@
+module Disconnect
+
+open C.String
+open Const
+
+module U8 = FStar.UInt8
+
+val assemble_disconnect_struct: s: struct_disconnect_parts
+  -> Pure struct_fixed_header
+    (requires true)
+    (ensures (fun r -> true))
+let assemble_disconnect_struct s =
+    let disconnect_constant: struct_fixed_header_constant = s.disconnect_disconnect_constant in
+    {
+      message_type = disconnect_constant.message_type_constant;
+      message_name = disconnect_constant.message_name_constant;
+      flags = {
+        flag = disconnect_constant.flags_constant.flag;
+        dup_flag = disconnect_constant.flags_constant.dup_flag;
+        qos_flag = disconnect_constant.flags_constant.qos_flag;
+        retain_flag = disconnect_constant.flags_constant.retain_flag;
+      };
+      remaining_length = s.disconnect_remaining_length;
+      connect = {
+        protocol_name = !$"";
+        protocol_version = max_u8;
+        flags = {
+          connect_flag = max_u8;
+          user_name = max_u8;
+          password = max_u8;
+          will_retain = max_u8;
+          will_qos = max_u8;
+          will_flag = max_u8;
+          clean_start = max_u8;
+        };
+        keep_alive = max_u32;
+        connect_topic_length = max_u32;
+        connect_property = {
+          connect_property_id = max_u8;
+          connect_property_name = !$"";
+        }
+      };
+      publish = {
+        topic_length = max_u32;
+        topic_name = !$"";
+        property_length = max_u32;
+        payload = !$"";
+      };
+      disconnect = (
+        if (U8.eq disconnect_constant.flags_constant.flag define_disconnect_reason_code_normal_disconnection) then
+          define_struct_disconnect_normal_disconnection
+
+        else if (U8.eq disconnect_constant.flags_constant.flag define_disconnect_reason_code_disconnect_with_will_message) then
+          define_struct_disconnect_disconnect_with_will_message
+
+        else if (U8.eq disconnect_constant.flags_constant.flag define_disconnect_reason_code_unspecified_error) then
+          define_struct_disconnect_unspecified_error
+
+        else if (U8.eq disconnect_constant.flags_constant.flag define_disconnect_reason_code_malformed_packet) then
+          define_struct_disconnect_malformed_packet
+
+        else if (U8.eq disconnect_constant.flags_constant.flag define_disconnect_reason_code_protocol_error) then
+          define_struct_disconnect_protocol_error
+
+        else if (U8.eq disconnect_constant.flags_constant.flag define_disconnect_reason_code_implementation_specific_error) then
+          define_struct_disconnect_implementation_specific_error
+
+        else if (U8.eq disconnect_constant.flags_constant.flag define_disconnect_reason_code_not_authorized) then
+          define_struct_disconnect_not_authorized
+
+        else if (U8.eq disconnect_constant.flags_constant.flag define_disconnect_reason_code_server_busy) then
+          define_struct_disconnect_server_busy
+
+        else if (U8.eq disconnect_constant.flags_constant.flag define_disconnect_reason_code_server_shutting_down) then
+          define_struct_disconnect_server_shutting_down
+
+        else if (U8.eq disconnect_constant.flags_constant.flag define_disconnect_reason_code_keep_alive_timeout) then
+            define_struct_disconnect_keep_alive_timeout
+
+        else if (U8.eq disconnect_constant.flags_constant.flag define_disconnect_reason_code_session_taken_over) then
+            define_struct_disconnect_session_taken_over
+            
+        else if (U8.eq disconnect_constant.flags_constant.flag define_disconnect_reason_code_topic_filter_invalid) then
+            define_struct_disconnect_topic_filter_invalid
+        else if (U8.eq disconnect_constant.flags_constant.flag define_disconnect_reason_code_topic_name_invalid) then
+            define_struct_disconnect_topic_name_invalid
+
+        else if (U8.eq disconnect_constant.flags_constant.flag define_disconnect_reason_receive_maximum_exceeded) then
+            define_struct_disconnect_receive_maximum_exceeded
+
+        else if (U8.eq disconnect_constant.flags_constant.flag define_disconnect_reason_topic_alias_invalid) then
+            define_struct_disconnect_topic_alias_invalid
+
+        else if (U8.eq disconnect_constant.flags_constant.flag define_disconnect_reason_packet_too_large) then
+            define_struct_disconnect_packet_too_large
+
+        else if (U8.eq disconnect_constant.flags_constant.flag define_disconnect_reason_message_rate_too_high) then
+            define_struct_disconnect_message_rate_too_high
+
+        else if (U8.eq disconnect_constant.flags_constant.flag define_disconnect_reason_quota_exceeded) then
+            define_struct_disconnect_quota_exceeded
+
+        else if (U8.eq disconnect_constant.flags_constant.flag define_disconnect_reason_administrative_action) then
+            define_struct_disconnect_administrative_action
+
+        else if (U8.eq disconnect_constant.flags_constant.flag define_disconnect_reason_payload_format_invalid) then
+            define_struct_disconnect_payload_format_invalid
+
+        else if (U8.eq disconnect_constant.flags_constant.flag define_disconnect_reason_retain_not_supported) then
+            define_struct_disconnect_retain_not_supported
+
+        else if (U8.eq disconnect_constant.flags_constant.flag define_disconnect_reason_qos_not_supported) then
+            define_struct_disconnect_qos_not_supported
+
+        else if (U8.eq disconnect_constant.flags_constant.flag define_disconnect_reason_use_another_server) then
+            define_struct_disconnect_use_another_server
+
+        else if (U8.eq disconnect_constant.flags_constant.flag define_disconnect_reason_server_moved) then
+            define_struct_disconnect_server_moved
+
+        else if (U8.eq disconnect_constant.flags_constant.flag define_disconnect_reason_shared_subscriptions_not_supported) then
+            define_struct_disconnect_shared_subscriptions_not_supported
+
+        else if (U8.eq disconnect_constant.flags_constant.flag define_disconnect_reason_connection_rate_exceeded) then
+            define_struct_disconnect_connection_rate_exceeded
+
+        else if (U8.eq disconnect_constant.flags_constant.flag define_disconnect_reason_maximum_connect_time) then
+            define_struct_disconnect_maximum_connect_time
+
+        else if (U8.eq disconnect_constant.flags_constant.flag define_disconnect_reason_subscription_identifiers_not_supported) then
+            define_struct_disconnect_subscription_identifiers_not_supported
+
+        else // if (U8.eq disconnect_constant.flags_constant.flag define_disconnect_reason_wildcard_subscriptions_not_supported) then
+            define_struct_disconnect_wildcard_subscriptions_not_supported
+      );
+
+      error = {
+        code = define_no_error_code;
+        message = define_no_error;
+      };
+    }
