src/mqtt-packet-parser/src/publish.fst
@@ -1,0 +1,103 @@
+module Publish
+
+module U8 = FStar.UInt8
+
+open C.String
+
+open Const
+open Common
+
+val get_dup_flag: fixed_header_first_one_byte: U8.t -> type_dup_flags_restrict
+let get_dup_flag fixed_header_first_one_byte =
+  let dup_flag_bits: U8.t = slice_byte fixed_header_first_one_byte 4uy 5uy in
+  if (U8.gt dup_flag_bits 1uy) then
+    max_u8
+  else
+    dup_flag_bits
+
+val get_qos_flag: fixed_header_first_one_byte: U8.t -> type_qos_flags_restrict
+let get_qos_flag fixed_header_first_one_byte =
+    let qos_flag_bits: U8.t = slice_byte fixed_header_first_one_byte 5uy 7uy in
+    if (U8.gt qos_flag_bits 2uy) then
+      max_u8
+    else
+      qos_flag_bits
+
+val get_retain_flag: fixed_header_first_one_byte: U8.t -> type_retain_flags_restrict
+let get_retain_flag fixed_header_first_one_byte =
+    let retain_flag_bits: U8.t = slice_byte fixed_header_first_one_byte 7uy 8uy in
+    if (U8.gt retain_flag_bits 1uy) then
+      max_u8
+    else
+      retain_flag_bits
+
+val struct_fixed_publish:
+  (dup_flag:type_dup_flags_restrict)
+  -> (qos_flag:type_qos_flags_restrict)
+  -> (retain_flag:type_retain_flags_restrict)
+  -> struct_fixed_header_constant
+let struct_fixed_publish dup_flag qos_flag retain_flag = {
+  message_type_constant = define_mqtt_control_packet_PUBLISH;
+  message_name_constant = define_mqtt_control_packet_PUBLISH_label;
+  flags_constant = {
+    flag = max_u8;
+    dup_flag = dup_flag;
+    qos_flag = qos_flag;
+    retain_flag = retain_flag;
+  };
+}
+
+val assemble_publish_struct: s: struct_publish_parts
+  -> Pure struct_fixed_header
+    (requires true)
+    (ensures (fun r -> true))
+let assemble_publish_struct s =
+      let dup_flag: type_dup_flags_restrict = get_dup_flag s.publish_fixed_header_first_one_byte in
+      let qos_flag: type_qos_flags_restrict = get_qos_flag s.publish_fixed_header_first_one_byte in
+      let retain_flag: type_retain_flags_restrict = get_retain_flag s.publish_fixed_header_first_one_byte in
+      let data: struct_fixed_header_constant =
+        struct_fixed_publish dup_flag qos_flag retain_flag in
+        {
+          message_type = data.message_type_constant;
+          message_name = data.message_name_constant;
+          flags = {
+            flag = data.flags_constant.flag;
+            dup_flag = data.flags_constant.dup_flag;
+            qos_flag = data.flags_constant.qos_flag;
+            retain_flag = data.flags_constant.retain_flag;
+          };
+          remaining_length = s.publish_remaining_length;
+          connect = {
+            protocol_name = !$"";
+            protocol_version = max_u8;
+            flags = {
+              connect_flag = max_u8;
+              user_name = max_u8;
+              password = max_u8;
+              will_retain = max_u8;
+              will_qos = max_u8;
+              will_flag = max_u8;
+              clean_start = max_u8;
+            };
+            keep_alive = max_u32;
+            connect_topic_length = max_u32;
+            connect_property = {
+              connect_property_id = max_u8;
+              connect_property_name = !$""
+            }
+          };
+          publish = {
+            topic_length = s.publish_topic_length;
+            topic_name = s.publish_topic_name;
+            property_length = s.publish_property_length;
+            payload = s.publish_payload;
+          };
+          disconnect = {
+            disconnect_reason_code = max_u8;
+            disconnect_reason_code_name = !$"";
+          };
+          error = {
+            code = define_no_error_code;
+            message = define_no_error;
+          };
+        }
